\documentclass[12pt]{article}

\usepackage{amsmath}
\usepackage{amssymb}

\begin{document}
    \begin{section}{Constant Zonal Flow}
        \begin{subsection}{Basic States}
            \begin{align*}
                &\Psi_1 = -U_1 y
                &\Psi_2 = -U_2 y \\
                &Q_1 = (U_1 - U_2 + \beta) y
                &Q_2 = (U_2 - U_1 + \beta) y
            \end{align*}
        \end{subsection}

        \begin{subsection}{New States and Perturbations}
            \begin{align*}
                 &\psi_1 = \Psi_1 + \psi_1'
                 &\psi_2 = \Psi_2 + \psi_2' \\
                 &q_1' = \nabla^2\psi_1' - F_1(\psi_1' - \psi_2')
                 &q_2' = \nabla^2\psi_2' - F_2(\psi_2' - \psi_1') \\
            \end{align*}
        \end{subsection}

        \begin{subsection}{QG Equations}
            \begin{align*}
                 0 &= \partial_t q_1' + (u_1' + U_1)\partial_x q_1' + v_1' \partial_y(q_1' + Q_1) \\
                 0 &= \partial_t q_2' + (u_2' + U_2)\partial_x q_2' + v_2' \partial_y(q_2' + Q_2) \\
            \end{align*}
        \end{subsection}

        \begin{subsection}{Normal Modes}
            \begin{align*}
                 &\hat{q_1'} = -\hat{\psi_1'}(F_1 + K^2) + F_1\hat{\psi_2'}
                 &\hat{q_2'} = F_2\hat{\psi_1'} - \hat{\psi_2'}(F_2 + K^2) \\
                &\hat{\psi_1'} = \frac{(F_2 + K^2) \hat{q_1'} + F_1\hat{q_2'}}{F_1F_2 - (F_1 + K^2)(F_2 + K^2)}
                &\hat{\psi_2'} = \frac{F_2\hat{q_1'} + (F_1 + K^2)\hat{q_2'}}{F_1F_2 - (F_1 + K^2)(F_2 + K^2)} \\
                &\hat{u_1'} = -ik \hat{\psi_1'}
                &\hat{u_2'} = -ik \hat{\psi_2'} \\
                &\hat{u_1'} = -il \hat{\psi_1'}
                &\hat{u_2'} = -il \hat{\psi_2'} \\
                &K^2 = k^2 + l^2
            \end{align*}
        \end{subsection}
    \end{section}

    \newpage
    \begin{section}{$x$-independent Zonal Flow}
        \begin{subsection}{Basic States}
            \begin{align*}
                &\Psi_1 = \Psi_1(y)
                &\Psi_2 = \Psi_2(y) \\
                &Q_1 = \partial_{yy}\Psi_1 - F_1(\Psi_1 - \Psi_2) + \beta y
                &Q_2 = \partial_{yy}\Psi_2 - F_2(\Psi_2 - \Psi_1) + \beta y
            \end{align*}
        \end{subsection}

        \begin{subsection}{New States and Perturbations}
            \begin{align*}
                 &\psi_1 = \Psi_1 + \psi_1'
                 &\psi_2 = \Psi_2 + \psi_2' \\
                 &q_1' = \nabla^2\psi_1' - F_1(\psi_1' - \psi_2')
                 &q_2' = \nabla^2\psi_2' - F_2(\psi_2' - \psi_1') \\
            \end{align*}
        \end{subsection}

        \begin{subsection}{QG Equations}
            \begin{align*}
                 0 &= \partial_t q_1' + (u_1' + U_1)\partial_x q_1' + v_1' \partial_y(q_1' + Q_1) \\
                 0 &= \partial_t q_2' + (u_2' + U_2)\partial_x q_2' + v_2' \partial_y(q_2' + Q_2) \\
            \end{align*}
        \end{subsection}

        \begin{subsection}{Normal Modes}
            \begin{align*}
                 &\hat{q_1'} = -\hat{\psi_1'}(F_1 + K^2) + F_1\hat{\psi_2'}
                 &\hat{q_2'} = F_2\hat{\psi_1'} - \hat{\psi_2'}(F_2 + K^2) \\
                &\hat{\psi_1'} = \frac{(F_2 + K^2) \hat{q_1'} + F_1\hat{q_2'}}{F_1F_2 - (F_1 + K^2)(F_2 + K^2)}
                &\hat{\psi_2'} = \frac{F_2\hat{q_1'} + (F_1 + K^2)\hat{q_2'}}{F_1F_2 - (F_1 + K^2)(F_2 + K^2)} \\
                &\hat{u_1'} = -ik \hat{\psi_1'}
                &\hat{u_2'} = -ik \hat{\psi_2'} \\
                &\hat{u_1'} = -il \hat{\psi_1'}
                &\hat{u_2'} = -il \hat{\psi_2'} \\
                &K^2 = k^2 + l^2
            \end{align*}
        \end{subsection}
    \end{section}

\end{document}
